## 

### 题目链接：



### 答案

#### 解法一

```Java
public class Solution {
    public int LastRemaining_Solution(int n, int m) {
        if(n == 0) return -1;
        if(n == 1) return 0;
        int y = 0;
        for(int i = 2; i <= n; ++i){
            y = (y + m) % i;
        }
        return y;
    }
}
```
#### 解法二

```Java
public class Solution {
    public int LastRemaining_Solution(int n, int m) {
        if(n == 0) return -1;
        if(n == 1) return 0;
        return (LastRemaining_Solution(n-1,m) + m) % n;
        
    }
}
```

#### 解法三

```Java

```
